@prefix owl:   <http://www.w3.org/2002/07/owl#> .
@prefix rdf:   <http://www.w3.org/1999/02/22-rdf-syntax-ns#> .
@prefix xsd:   <http://www.w3.org/2001/XMLSchema#> .
@prefix rdfs:  <http://www.w3.org/2000/01/rdf-schema#> .

<http://lbd.arch.rwth-aachen.de/bcf/v2.1/hasAuthoringToolId>
        a             owl:ObjectProperty ;
        rdfs:comment  "Name of the system in which the component is originated"@en ;
        rdfs:domain   <http://lbd.arch.rwth-aachen.de/bcf/v2.1/Component> .

<http://lbd.arch.rwth-aachen.de/bcf/v2.1/DocumentReference>
        a                owl:Class ;
        rdfs:comment     "DocumentReference provides a means to associate additional payloads or links with topics. The references may point to a file within the .bcfzip or to an external location."@en ;
        rdfs:subClassOf  [ a                   owl:Restriction ;
                           owl:minCardinality  "0"^^xsd:int ;
                           owl:onProperty      <http://lbd.arch.rwth-aachen.de/bcf/v2.1/hasDescription>
                         ] ;
        rdfs:subClassOf  [ a                   owl:Restriction ;
                           owl:minCardinality  "0"^^xsd:int ;
                           owl:onProperty      <http://lbd.arch.rwth-aachen.de/bcf/v2.1/hasReferencedDocument>
                         ] ;
        rdfs:subClassOf  [ a                   owl:Restriction ;
                           owl:maxCardinality  "1"^^xsd:int ;
                           owl:onProperty      <http://lbd.arch.rwth-aachen.de/bcf/v2.1/hasDocumentReferenceGuid>
                         ] ;
        rdfs:subClassOf  [ a                   owl:Restriction ;
                           owl:minCardinality  "0"^^xsd:int ;
                           owl:onProperty      <http://lbd.arch.rwth-aachen.de/bcf/v2.1/hasDocumentReferenceGuid>
                         ] .

<http://lbd.arch.rwth-aachen.de/bcf/v2.1/PerspectiveCamera>
        a                owl:Class ;
        rdfs:comment     "This element describes a viewpoint using perspective camera."@en ;
        rdfs:subClassOf  <http://lbd.arch.rwth-aachen.de/bcf/v2.1/Camera> ;
        rdfs:subClassOf  [ a                   owl:Restriction ;
                           owl:minCardinality  "1"^^xsd:int ;
                           owl:onProperty      <http://lbd.arch.rwth-aachen.de/bcf/v2.1/hasFieldOfView>
                         ] .

<http://lbd.arch.rwth-aachen.de/bcf/v2.1/hasDocumentReference>
        a            owl:ObjectProperty ;
        rdfs:domain  <http://lbd.arch.rwth-aachen.de/bcf/v2.1/Markup> ;
        rdfs:range   <http://lbd.arch.rwth-aachen.de/bcf/v2.1/DocumentReference> .

<http://lbd.arch.rwth-aachen.de/bcf/v2.1/hasCommentDate>
        a             owl:DatatypeProperty ;
        rdfs:comment  "Date of the comment"@en ;
        rdfs:domain   <http://lbd.arch.rwth-aachen.de/bcf/v2.1/Comment> ;
        rdfs:range    xsd:dateTime .

<http://lbd.arch.rwth-aachen.de/bcf/v2.1/hasProject >
        a            owl:ObjectProperty ;
        rdfs:domain  <http://lbd.arch.rwth-aachen.de/bcf/v2.1/BCF> ;
        rdfs:range   <http://lbd.arch.rwth-aachen.de/bcf/v2.1/Project > .

<http://lbd.arch.rwth-aachen.de/bcf/v2.1/hasReferenceLink>
        a             owl:ObjectProperty ;
        rdfs:comment  "List of references to the topic, for example, a work request management system or an URI to a model."@en ;
        rdfs:domain   <http://lbd.arch.rwth-aachen.de/bcf/v2.1/Topic> .

<http://lbd.arch.rwth-aachen.de/bcf/v2.1/hasTopicType>
        a             owl:ObjectProperty ;
        rdfs:comment  "Type of the topic (Predefined list)"@en ;
        rdfs:domain   <http://lbd.arch.rwth-aachen.de/bcf/v2.1/Topic> .

<http://lbd.arch.rwth-aachen.de/bcf/v2.1/hasFileDate>
        a            owl:ObjectProperty ;
        rdfs:domain  <http://lbd.arch.rwth-aachen.de/bcf/v2.1/Header> .

<http://lbd.arch.rwth-aachen.de/bcf/v2.1/hasTopicStatus>
        a             owl:ObjectProperty ;
        rdfs:comment  "Type of the topic (Predefined list)"@en ;
        rdfs:domain   <http://lbd.arch.rwth-aachen.de/bcf/v2.1/Topic> .

<http://lbd.arch.rwth-aachen.de/bcf/v2.1/hasPerspectiveCamera>
        a            owl:ObjectProperty ;
        rdfs:domain  <http://lbd.arch.rwth-aachen.de/bcf/v2.1/VisualizationInfo> ;
        rdfs:range   <http://lbd.arch.rwth-aachen.de/bcf/v2.1/PerspectiveCamera> .

<http://lbd.arch.rwth-aachen.de/bcf/v2.1/hasComponent>
        a            owl:ObjectProperty ;
        rdfs:domain  <http://lbd.arch.rwth-aachen.de/bcf/v2.1/Selection> ;
        rdfs:range   <http://lbd.arch.rwth-aachen.de/bcf/v2.1/Component> .

<http://lbd.arch.rwth-aachen.de/bcf/v2.1/hasViewSetupHints>
        a            owl:ObjectProperty ;
        rdfs:domain  <http://lbd.arch.rwth-aachen.de/bcf/v2.1/Components> ;
        rdfs:range   <http://lbd.arch.rwth-aachen.de/bcf/v2.1/ViewSetupHints> .

<http://lbd.arch.rwth-aachen.de/bcf/v2.1/OrthogonalCamera>
        a                owl:Class ;
        rdfs:comment     "This element describes a viewpoint using orthogonal camera. "@en ;
        rdfs:subClassOf  <http://lbd.arch.rwth-aachen.de/bcf/v2.1/Camera> ;
        rdfs:subClassOf  [ a                   owl:Restriction ;
                           owl:minCardinality  "1"^^xsd:int ;
                           owl:onProperty      <http://lbd.arch.rwth-aachen.de/bcf/v2.1/hasViewToWorldScale>
                         ] .

<http://lbd.arch.rwth-aachen.de/bcf/v2.1/hasReference>
        a             owl:ObjectProperty ;
        rdfs:comment  "URI to BimSnippet IFC."@en ;
        rdfs:domain   <http://lbd.arch.rwth-aachen.de/bcf/v2.1/BimSnippet> .

<http://lbd.arch.rwth-aachen.de/bcf/v2.1/hasIndex>
        a             owl:DatatypeProperty , owl:ObjectProperty ;
        rdfs:comment  "Parameter for sorting"@en , "Number to maintain the order of the topics."@en ;
        rdfs:domain   <http://lbd.arch.rwth-aachen.de/bcf/v2.1/Viewpoints> , <http://lbd.arch.rwth-aachen.de/bcf/v2.1/Topic> ;
        rdfs:range    xsd:integer .

<http://lbd.arch.rwth-aachen.de/bcf/v2.1/hasVisibility>
        a            owl:ObjectProperty ;
        rdfs:domain  <http://lbd.arch.rwth-aachen.de/bcf/v2.1/Components> ;
        rdfs:range   <http://lbd.arch.rwth-aachen.de/bcf/v2.1/Visibility> .

<http://lbd.arch.rwth-aachen.de/bcf/v2.1/hasReferenceSchema>
        a             owl:ObjectProperty ;
        rdfs:comment  "URI to BimSnippetSchema"@en ;
        rdfs:domain   <http://lbd.arch.rwth-aachen.de/bcf/v2.1/BimSnippet> .

<http://lbd.arch.rwth-aachen.de/bcf/v2.1/Components>
        a             owl:Class ;
        rdfs:comment  "The components node contains a set of Component references. The numeric values in this file are all given in fixed units (meters for length and degrees for angle). Unit conversion is not required, since the values are not relevant to the user. The components node has also the DefaultVisibility attribute which indicates true or false for all components of the viewpoint."@en .

<http://lbd.arch.rwth-aachen.de/bcf/v2.1/hasIfcSpatialStructureElement>
        a             owl:DatatypeProperty ;
        rdfs:comment  "IfcGuid Reference to the spatial structure element, e.g. IfcBuildingStorey, to which this topic is related."@en ;
        rdfs:domain   <http://lbd.arch.rwth-aachen.de/bcf/v2.1/Header> .

<http://lbd.arch.rwth-aachen.de/bcf/v2.1/hasLines>
        a            owl:ObjectProperty ;
        rdfs:domain  <http://lbd.arch.rwth-aachen.de/bcf/v2.1/VisualizationInfo> ;
        rdfs:range   <http://lbd.arch.rwth-aachen.de/bcf/v2.1/Lines> .

<http://lbd.arch.rwth-aachen.de/bcf/v2.1/Topic>
        a                owl:Class ;
        rdfs:comment     "Topic node contains reference information of the topic. It has one attribute, Guid, which is the topic GUID."@en ;
        rdfs:subClassOf  [ a                   owl:Restriction ;
                           owl:minCardinality  "0"^^xsd:int ;
                           owl:onProperty      <http://lbd.arch.rwth-aachen.de/bcf/v2.1/hasTopicType>
                         ] ;
        rdfs:subClassOf  [ a                   owl:Restriction ;
                           owl:minCardinality  "1"^^xsd:int ;
                           owl:onProperty      <http://lbd.arch.rwth-aachen.de/bcf/v2.1/hasTopicGuid>
                         ] ;
        rdfs:subClassOf  [ a                   owl:Restriction ;
                           owl:minCardinality  "1"^^xsd:int ;
                           owl:onProperty      <http://lbd.arch.rwth-aachen.de/bcf/v2.1/hasTitle>
                         ] ;
        rdfs:subClassOf  [ a                   owl:Restriction ;
                           owl:minCardinality  "0"^^xsd:int ;
                           owl:onProperty      <http://lbd.arch.rwth-aachen.de/bcf/v2.1/hasLabels>
                         ] ;
        rdfs:subClassOf  [ a                   owl:Restriction ;
                           owl:minCardinality  "0"^^xsd:int ;
                           owl:onProperty      <http://lbd.arch.rwth-aachen.de/bcf/v2.1/hasModifiedAuthor>
                         ] ;
        rdfs:subClassOf  [ a                   owl:Restriction ;
                           owl:minCardinality  "0"^^xsd:int ;
                           owl:onProperty      <http://lbd.arch.rwth-aachen.de/bcf/v2.1/hasPriority>
                         ] ;
        rdfs:subClassOf  [ a                   owl:Restriction ;
                           owl:minCardinality  "0"^^xsd:int ;
                           owl:onProperty      <http://lbd.arch.rwth-aachen.de/bcf/v2.1/hasStage>
                         ] ;
        rdfs:subClassOf  [ a                   owl:Restriction ;
                           owl:minCardinality  "0"^^xsd:int ;
                           owl:onProperty      <http://lbd.arch.rwth-aachen.de/bcf/v2.1/hasIndex>
                         ] ;
        rdfs:subClassOf  [ a                   owl:Restriction ;
                           owl:minCardinality  "0"^^xsd:int ;
                           owl:onProperty      <http://lbd.arch.rwth-aachen.de/bcf/v2.1/hasReferenceLink>
                         ] ;
        rdfs:subClassOf  [ a                   owl:Restriction ;
                           owl:maxCardinality  "1"^^xsd:int ;
                           owl:onProperty      <http://lbd.arch.rwth-aachen.de/bcf/v2.1/hasTopicGuid>
                         ] ;
        rdfs:subClassOf  [ a                   owl:Restriction ;
                           owl:minCardinality  "1"^^xsd:int ;
                           owl:onProperty      <http://lbd.arch.rwth-aachen.de/bcf/v2.1/hasCreationDate>
                         ] ;
        rdfs:subClassOf  [ a                   owl:Restriction ;
                           owl:minCardinality  "1"^^xsd:int ;
                           owl:onProperty      <http://lbd.arch.rwth-aachen.de/bcf/v2.1/hasCreationAuthor>
                         ] ;
        rdfs:subClassOf  [ a                   owl:Restriction ;
                           owl:maxCardinality  "1"^^xsd:int ;
                           owl:onProperty      <http://lbd.arch.rwth-aachen.de/bcf/v2.1/hasTopicType>
                         ] ;
        rdfs:subClassOf  [ a                   owl:Restriction ;
                           owl:maxCardinality  "1"^^xsd:int ;
                           owl:onProperty      <http://lbd.arch.rwth-aachen.de/bcf/v2.1/hasTopicStatus>
                         ] ;
        rdfs:subClassOf  [ a                   owl:Restriction ;
                           owl:minCardinality  "0"^^xsd:int ;
                           owl:onProperty      <http://lbd.arch.rwth-aachen.de/bcf/v2.1/hasDescription>
                         ] ;
        rdfs:subClassOf  [ a                   owl:Restriction ;
                           owl:minCardinality  "0"^^xsd:int ;
                           owl:onProperty      <http://lbd.arch.rwth-aachen.de/bcf/v2.1/hasModifiedDate>
                         ] ;
        rdfs:subClassOf  [ a                   owl:Restriction ;
                           owl:minCardinality  "0"^^xsd:int ;
                           owl:onProperty      <http://lbd.arch.rwth-aachen.de/bcf/v2.1/hasTopicStatus>
                         ] ;
        rdfs:subClassOf  [ a                   owl:Restriction ;
                           owl:minCardinality  "0"^^xsd:int ;
                           owl:onProperty      <http://lbd.arch.rwth-aachen.de/bcf/v2.1/hasAssignedTo>
                         ] ;
        rdfs:subClassOf  [ a                   owl:Restriction ;
                           owl:minCardinality  "0"^^xsd:int ;
                           owl:onProperty      <http://lbd.arch.rwth-aachen.de/bcf/v2.1/hasDueDate>
                         ] .

<http://lbd.arch.rwth-aachen.de/bcf/v2.1/hasDocumentReferenceGuid>
        a             owl:DatatypeProperty ;
        rdfs:comment  "Guid attribute for identifying it uniquely"@en ;
        rdfs:domain   <http://lbd.arch.rwth-aachen.de/bcf/v2.1/DocumentReference> ;
        rdfs:range    xsd:string .

<http://lbd.arch.rwth-aachen.de/bcf/v2.1/hasSnapshot>
        a             owl:ObjectProperty ;
        rdfs:comment  "The URL of the snapshot(.png)"@en ;
        rdfs:domain   <http://lbd.arch.rwth-aachen.de/bcf/v2.1/Viewpoints> .

<http://lbd.arch.rwth-aachen.de/bcf/v2.1/hasBimSnippet>
        a            owl:ObjectProperty ;
        rdfs:domain  <http://lbd.arch.rwth-aachen.de/bcf/v2.1/Markup> ;
        rdfs:range   <http://lbd.arch.rwth-aachen.de/bcf/v2.1/BimSnippet> .

<http://lbd.arch.rwth-aachen.de/bcf/v2.1/hasViewpoints>
        a            owl:ObjectProperty ;
        rdfs:domain  <http://lbd.arch.rwth-aachen.de/bcf/v2.1/Markup> ;
        rdfs:range   <http://lbd.arch.rwth-aachen.de/bcf/v2.1/Viewpoints> .

<http://lbd.arch.rwth-aachen.de/bcf/v2.1/hasMarkup>
        a            owl:ObjectProperty ;
        rdfs:domain  <http://lbd.arch.rwth-aachen.de/bcf/v2.1/BCF> ;
        rdfs:range   <http://lbd.arch.rwth-aachen.de/bcf/v2.1/Markup> .

<http://lbd.arch.rwth-aachen.de/bcf/v2.1/Coloring>
        a             owl:Class ;
        rdfs:comment  "The Coloring element lists colors and a list of associated components that should be displayed with the specified color when displaying a viewpoint. The color is given in ARGB format. Colors are represented as 6 or 8 hexadecimal digits. If 8 digits are present, the first two represent the alpha (transparency) channel. For example, 40E0D0 would be the color <span style=\"color:#40E0D0;\";>Turquoise. More information about the color format can be found on Wikipedia."@en .

<http://lbd.arch.rwth-aachen.de/bcf/v2.1/hasIfcGuid>
        a             owl:ObjectProperty ;
        rdfs:comment  "The IfcGuid of the component"@en ;
        rdfs:domain   <http://lbd.arch.rwth-aachen.de/bcf/v2.1/Component> .

<http://lbd.arch.rwth-aachen.de/bcf/v2.1/hasColoring>
        a            owl:ObjectProperty ;
        rdfs:domain  <http://lbd.arch.rwth-aachen.de/bcf/v2.1/Components> ;
        rdfs:range   <http://lbd.arch.rwth-aachen.de/bcf/v2.1/Coloring> .

<http://lbd.arch.rwth-aachen.de/bcf/v2.1/ClippingPlanes>
        a             owl:Class ;
        rdfs:comment  "ClippingPlanes can be used to define a subsection of a building model that is related to the topic. Each clipping plane is defined by Location and Direction."@en .

<http://lbd.arch.rwth-aachen.de/bcf/v2.1/hasViewpoint>
        a             owl:ObjectProperty ;
        rdfs:comment  "The viewpoint "@en , "Back reference to the viewpoint"@en ;
        rdfs:domain   <http://lbd.arch.rwth-aachen.de/bcf/v2.1/Viewpoints> , <http://lbd.arch.rwth-aachen.de/bcf/v2.1/Comment> .

<http://lbd.arch.rwth-aachen.de/bcf/v2.1/hasName>
        a             owl:DatatypeProperty ;
        rdfs:comment  "Name of the project."@en ;
        rdfs:domain   <http://lbd.arch.rwth-aachen.de/bcf/v2.1/Project > ;
        rdfs:range    xsd:string .

<http://lbd.arch.rwth-aachen.de/bcf/v2.1/hasStage>
        a             owl:ObjectProperty ;
        rdfs:comment  "Stage this topic is part of (Predefined list)."@en ;
        rdfs:domain   <http://lbd.arch.rwth-aachen.de/bcf/v2.1/Topic> .

<http://lbd.arch.rwth-aachen.de/bcf/v2.1/hasViewToWorldScale>
        a             owl:ObjectProperty ;
        rdfs:comment  "Scaling from view to world"@en ;
        rdfs:domain   <http://lbd.arch.rwth-aachen.de/bcf/v2.1/OrthogonalCamera> .

<http://lbd.arch.rwth-aachen.de/bcf/v2.1/Selection>
        a             owl:Class ;
        rdfs:comment  "The Selection element lists all components that should be either highlighted or selected when displaying a viewpoint."@en .

<http://lbd.arch.rwth-aachen.de/bcf/v2.1/hasRelatedTopic>
        a             owl:ObjectProperty ;
        rdfs:comment  " GUID of the referenced topic"@en ;
        rdfs:domain   <http://lbd.arch.rwth-aachen.de/bcf/v2.1/RelatedTopic> , <http://lbd.arch.rwth-aachen.de/bcf/v2.1/Markup> ;
        rdfs:range    <http://lbd.arch.rwth-aachen.de/bcf/v2.1/RelatedTopic> .

<http://lbd.arch.rwth-aachen.de/bcf/v2.1/hasCameraViewPoint>
        a             owl:ObjectProperty ;
        rdfs:comment  "\tCamera location"@en ;
        rdfs:domain   <http://lbd.arch.rwth-aachen.de/bcf/v2.1/Camera> .

<http://lbd.arch.rwth-aachen.de/bcf/v2.1/BimSnippet>
        a                owl:Class ;
        rdfs:comment     "BimSnippet is an additional file containing information related to one or multiple topics. For example, it can be an IFC file containing provisions for voids."@en ;
        rdfs:subClassOf  [ a                   owl:Restriction ;
                           owl:minCardinality  "0"^^xsd:int ;
                           owl:onProperty      <http://lbd.arch.rwth-aachen.de/bcf/v2.1/hasReferenceSchema>
                         ] ;
        rdfs:subClassOf  [ a                   owl:Restriction ;
                           owl:minCardinality  "1"^^xsd:int ;
                           owl:onProperty      <http://lbd.arch.rwth-aachen.de/bcf/v2.1/hasReference>
                         ] ;
        rdfs:subClassOf  [ a                   owl:Restriction ;
                           owl:maxCardinality  "1"^^xsd:int ;
                           owl:onProperty      <http://lbd.arch.rwth-aachen.de/bcf/v2.1/hasSnippetType>
                         ] ;
        rdfs:subClassOf  [ a                   owl:Restriction ;
                           owl:minCardinality  "1"^^xsd:int ;
                           owl:onProperty      <http://lbd.arch.rwth-aachen.de/bcf/v2.1/hasSnippetType>
                         ] .

<http://lbd.arch.rwth-aachen.de/bcf/v2.1/Viewpoints>
        a                owl:Class ;
        rdfs:comment     "The markup file can contain multiple viewpoints related to one or more comments. A viewpoint has also the Guid attribute for identifying it uniquely."@en ;
        rdfs:subClassOf  [ a                   owl:Restriction ;
                           owl:minCardinality  "0"^^xsd:int ;
                           owl:onProperty      <http://lbd.arch.rwth-aachen.de/bcf/v2.1/hasIndex>
                         ] ;
        rdfs:subClassOf  [ a                   owl:Restriction ;
                           owl:minCardinality  "0"^^xsd:int ;
                           owl:onProperty      <http://lbd.arch.rwth-aachen.de/bcf/v2.1/hasSnapshot>
                         ] ;
        rdfs:subClassOf  [ a                   owl:Restriction ;
                           owl:minCardinality  "0"^^xsd:int ;
                           owl:onProperty      <http://lbd.arch.rwth-aachen.de/bcf/v2.1/hasViewpoint>
                         ] .

<http://lbd.arch.rwth-aachen.de/bcf/v2.1/hasBitmap>
        a            owl:ObjectProperty ;
        rdfs:domain  <http://lbd.arch.rwth-aachen.de/bcf/v2.1/VisualizationInfo> ;
        rdfs:range   <http://lbd.arch.rwth-aachen.de/bcf/v2.1/Bitmap> .

<http://lbd.arch.rwth-aachen.de/bcf/v2.1/ViewSetupHints>
        a             owl:Class ;
        rdfs:comment  "This element contains information about the default visibility for elements of certain types (SpacesVisible, SpaceBoundariesVisible and OpeningsVisible) that should be applied if not stated otherwise."@en .

<http://lbd.arch.rwth-aachen.de/bcf/v2.1/hasTitle>
        a             owl:ObjectProperty ;
        rdfs:comment  "Title of the topic."@en ;
        rdfs:domain   <http://lbd.arch.rwth-aachen.de/bcf/v2.1/Topic> .

<http://lbd.arch.rwth-aachen.de/bcf/v2.1/Header>
        a                owl:Class ;
        rdfs:comment     "Header node contains information about the IFC files relevant to this topic. It has one attribute, ProjectGuid, which is the project GUID. Header has also a list of File nodes."@en ;
        rdfs:subClassOf  [ a                   owl:Restriction ;
                           owl:maxCardinality  "1"^^xsd:int ;
                           owl:onProperty      <http://lbd.arch.rwth-aachen.de/bcf/v2.1/hasFileDate>
                         ] ;
        rdfs:subClassOf  [ a                   owl:Restriction ;
                           owl:minCardinality  "0"^^xsd:int ;
                           owl:onProperty      <http://lbd.arch.rwth-aachen.de/bcf/v2.1/hasIfcProject>
                         ] ;
        rdfs:subClassOf  [ a                   owl:Restriction ;
                           owl:minCardinality  "0"^^xsd:int ;
                           owl:onProperty      <http://lbd.arch.rwth-aachen.de/bcf/v2.1/hasIfcSpatialStructureElement>
                         ] ;
        rdfs:subClassOf  [ a                   owl:Restriction ;
                           owl:minCardinality  "0"^^xsd:int ;
                           owl:onProperty      <http://lbd.arch.rwth-aachen.de/bcf/v2.1/hasFileDate>
                         ] ;
        rdfs:subClassOf  [ a                   owl:Restriction ;
                           owl:maxCardinality  "1"^^xsd:int ;
                           owl:onProperty      <http://lbd.arch.rwth-aachen.de/bcf/v2.1/hasIfcProject>
                         ] ;
        rdfs:subClassOf  [ a                   owl:Restriction ;
                           owl:maxCardinality  "1"^^xsd:int ;
                           owl:onProperty      <http://lbd.arch.rwth-aachen.de/bcf/v2.1/hasFileReference>
                         ] ;
        rdfs:subClassOf  [ a                   owl:Restriction ;
                           owl:maxCardinality  "1"^^xsd:int ;
                           owl:onProperty      <http://lbd.arch.rwth-aachen.de/bcf/v2.1/hasIfcSpatialStructureElement>
                         ] ;
        rdfs:subClassOf  [ a                   owl:Restriction ;
                           owl:minCardinality  "0"^^xsd:int ;
                           owl:onProperty      <http://lbd.arch.rwth-aachen.de/bcf/v2.1/hasFileReference>
                         ] .

<http://lbd.arch.rwth-aachen.de/bcf/v2.1/BCF>
        a             owl:Class ;
        rdfs:comment  "The markup contains textual information about the topic."@en .

<http://lbd.arch.rwth-aachen.de/bcf/v2.1/hasDueDate>
        a             owl:DatatypeProperty ;
        rdfs:comment  "Date until when the topics issue needs to be resolved."@en ;
        rdfs:domain   <http://lbd.arch.rwth-aachen.de/bcf/v2.1/Topic> ;
        rdfs:range    xsd:dateTime .

<http://lbd.arch.rwth-aachen.de/bcf/v2.1/hasPriority>
        a             owl:ObjectProperty ;
        rdfs:comment  "Topic priority. The list of possible values are defined in the extension schema."@en ;
        rdfs:domain   <http://lbd.arch.rwth-aachen.de/bcf/v2.1/Topic> .

<http://lbd.arch.rwth-aachen.de/bcf/v2.1/hasProjectId>
        a             owl:DatatypeProperty ;
        rdfs:comment  "ProjectId of the project"@en ;
        rdfs:domain   <http://lbd.arch.rwth-aachen.de/bcf/v2.1/Project > ;
        rdfs:range    xsd:string .

<http://lbd.arch.rwth-aachen.de/bcf/v2.1/hasCameraDirection>
        a             owl:ObjectProperty ;
        rdfs:comment  "Camera direction"@en ;
        rdfs:domain   <http://lbd.arch.rwth-aachen.de/bcf/v2.1/Camera> .

<http://lbd.arch.rwth-aachen.de/bcf/v2.1/Visibility>
        a             owl:Class ;
        rdfs:comment  "The Visibility element states the components DefaultVisibility and lists all Exceptions that apply to specific components."@en .

<http://lbd.arch.rwth-aachen.de/bcf/v2.1/hasExtensionSchema>
        a             owl:ObjectProperty ;
        rdfs:comment  "URI to the extension schema."@en ;
        rdfs:domain   <http://lbd.arch.rwth-aachen.de/bcf/v2.1/Project > .

<http://lbd.arch.rwth-aachen.de/bcf/v2.1/hasSelection>
        a            owl:ObjectProperty ;
        rdfs:domain  <http://lbd.arch.rwth-aachen.de/bcf/v2.1/Components> ;
        rdfs:range   <http://lbd.arch.rwth-aachen.de/bcf/v2.1/Selection> .

<http://lbd.arch.rwth-aachen.de/bcf/v2.1/hasLabels>
        a             owl:ObjectProperty ;
        rdfs:comment  "Tags for grouping Topics. The list of possible values are defined in the extension schema."@en ;
        rdfs:domain   <http://lbd.arch.rwth-aachen.de/bcf/v2.1/Topic> .

<http://lbd.arch.rwth-aachen.de/bcf/v2.1/hasSnippetType>
        a             owl:ObjectProperty ;
        rdfs:comment  "Type of the Snippet (Predefined listâ€�)"@en ;
        rdfs:domain   <http://lbd.arch.rwth-aachen.de/bcf/v2.1/BimSnippet> .

<http://lbd.arch.rwth-aachen.de/bcf/v2.1/hasModifiedAuthor>
        a             owl:ObjectProperty ;
        rdfs:comment  "The author who modified the comment"@en , "User who modified the topic. Exists only when Topic has been modified after creation."@en ;
        rdfs:domain   <http://lbd.arch.rwth-aachen.de/bcf/v2.1/Comment> , <http://lbd.arch.rwth-aachen.de/bcf/v2.1/Topic> .

<http://lbd.arch.rwth-aachen.de/bcf/v2.1/hasTopic>
        a            owl:ObjectProperty ;
        rdfs:domain  <http://lbd.arch.rwth-aachen.de/bcf/v2.1/Markup> ;
        rdfs:range   <http://lbd.arch.rwth-aachen.de/bcf/v2.1/Topic> .

<http://lbd.arch.rwth-aachen.de/bcf/v2.1/hasIfcProject>
        a             owl:DatatypeProperty ;
        rdfs:comment  "IfcGuid Reference to the project to which this topic is related in the IFC file"@en ;
        rdfs:domain   <http://lbd.arch.rwth-aachen.de/bcf/v2.1/Header> ;
        rdfs:range    xsd:string .

<http://lbd.arch.rwth-aachen.de/bcf/v2.1/hasCreationDate>
        a             owl:DatatypeProperty ;
        rdfs:comment  "Date when the topic was created."@en ;
        rdfs:domain   <http://lbd.arch.rwth-aachen.de/bcf/v2.1/Topic> ;
        rdfs:range    xsd:dateTime .

<http://lbd.arch.rwth-aachen.de/bcf/v2.1/hasComment>
        a             owl:DatatypeProperty , owl:ObjectProperty ;
        rdfs:comment  "The comment text"@en ;
        rdfs:domain   <http://lbd.arch.rwth-aachen.de/bcf/v2.1/Comment> , <http://lbd.arch.rwth-aachen.de/bcf/v2.1/Markup> ;
        rdfs:range    xsd:string , <http://lbd.arch.rwth-aachen.de/bcf/v2.1/Comment> .

<http://lbd.arch.rwth-aachen.de/bcf/v2.1/hasAssignedTo>
        a             owl:ObjectProperty ;
        rdfs:comment  "\tThe user to whom this topic is assigned to. Recommended to be in email format. The list of possible values are defined in the extension schema."@en ;
        rdfs:domain   <http://lbd.arch.rwth-aachen.de/bcf/v2.1/Topic> .

<http://lbd.arch.rwth-aachen.de/bcf/v2.1/hasCreationAuthor>
        a             owl:ObjectProperty ;
        rdfs:comment  "User who created the topic."@en ;
        rdfs:domain   <http://lbd.arch.rwth-aachen.de/bcf/v2.1/Topic> .

<http://lbd.arch.rwth-aachen.de/bcf/v2.1/Bitmap>
        a             owl:Class ;
        rdfs:comment  "A list of bitmaps can be used to add more information, for example, text in the visualization."@en .

<http://lbd.arch.rwth-aachen.de/bcf/v2.1/hasTopicGuid>
        a             owl:DatatypeProperty ;
        rdfs:comment  "Guid of the topic"@en ;
        rdfs:domain   <http://lbd.arch.rwth-aachen.de/bcf/v2.1/Topic> ;
        rdfs:range    xsd:string .

<http://lbd.arch.rwth-aachen.de/bcf/v2.1/Comment>
        a                owl:Class ;
        rdfs:comment     "The markup file can contain comments related to the topic. Their purpose is to record discussion between different parties related to the topic. Comment has also the Guid attribute for identifying it uniquely."@en ;
        rdfs:subClassOf  [ a                   owl:Restriction ;
                           owl:minCardinality  "0"^^xsd:int ;
                           owl:onProperty      <http://lbd.arch.rwth-aachen.de/bcf/v2.1/hasModifiedAuthor>
                         ] ;
        rdfs:subClassOf  [ a                   owl:Restriction ;
                           owl:minCardinality  "0"^^xsd:int ;
                           owl:onProperty      <http://lbd.arch.rwth-aachen.de/bcf/v2.1/hasModifiedDate>
                         ] ;
        rdfs:subClassOf  [ a                   owl:Restriction ;
                           owl:maxCardinality  "1"^^xsd:int ;
                           owl:onProperty      <http://lbd.arch.rwth-aachen.de/bcf/v2.1/hasCommentDate>
                         ] ;
        rdfs:subClassOf  [ a                   owl:Restriction ;
                           owl:minCardinality  "1"^^xsd:int ;
                           owl:onProperty      <http://lbd.arch.rwth-aachen.de/bcf/v2.1/hasAuthor>
                         ] ;
        rdfs:subClassOf  [ a                   owl:Restriction ;
                           owl:minCardinality  "1"^^xsd:int ;
                           owl:onProperty      <http://lbd.arch.rwth-aachen.de/bcf/v2.1/hasComment>
                         ] ;
        rdfs:subClassOf  [ a                   owl:Restriction ;
                           owl:maxCardinality  "1"^^xsd:int ;
                           owl:onProperty      <http://lbd.arch.rwth-aachen.de/bcf/v2.1/hasComment>
                         ] ;
        rdfs:subClassOf  [ a                   owl:Restriction ;
                           owl:minCardinality  "1"^^xsd:int ;
                           owl:onProperty      <http://lbd.arch.rwth-aachen.de/bcf/v2.1/hasCommentDate>
                         ] ;
        rdfs:subClassOf  [ a                   owl:Restriction ;
                           owl:minCardinality  "0"^^xsd:int ;
                           owl:onProperty      <http://lbd.arch.rwth-aachen.de/bcf/v2.1/hasViewpoint>
                         ] .

<http://lbd.arch.rwth-aachen.de/bcf/v2.1/RelatedTopic>
        a                owl:Class ;
        rdfs:comment     "Relation between topics (Clash -> PfV -> Opening)"@en ;
        rdfs:subClassOf  [ a                   owl:Restriction ;
                           owl:minCardinality  "0"^^xsd:int ;
                           owl:onProperty      <http://lbd.arch.rwth-aachen.de/bcf/v2.1/hasRelatedTopic>
                         ] .

<http://lbd.arch.rwth-aachen.de/bcf/v2.1/hasClippingPlanes>
        a            owl:ObjectProperty ;
        rdfs:domain  <http://lbd.arch.rwth-aachen.de/bcf/v2.1/VisualizationInfo> ;
        rdfs:range   <http://lbd.arch.rwth-aachen.de/bcf/v2.1/ClippingPlanes> .

<http://lbd.arch.rwth-aachen.de/bcf/v2.1/hasComponents>
        a            owl:ObjectProperty ;
        rdfs:domain  <http://lbd.arch.rwth-aachen.de/bcf/v2.1/VisualizationInfo> ;
        rdfs:range   <http://lbd.arch.rwth-aachen.de/bcf/v2.1/Components> .

<http://lbd.arch.rwth-aachen.de/bcf/v2.1/Project >
        a                owl:Class ;
        rdfs:comment     "The project contains reference information about the project the topics belong to."@en ;
        rdfs:subClassOf  [ a                   owl:Restriction ;
                           owl:minCardinality  "1"^^xsd:int ;
                           owl:onProperty      <http://lbd.arch.rwth-aachen.de/bcf/v2.1/hasExtensionSchema>
                         ] ;
        rdfs:subClassOf  [ a                   owl:Restriction ;
                           owl:minCardinality  "0"^^xsd:int ;
                           owl:onProperty      <http://lbd.arch.rwth-aachen.de/bcf/v2.1/hasName>
                         ] ;
        rdfs:subClassOf  [ a                   owl:Restriction ;
                           owl:maxCardinality  "1"^^xsd:int ;
                           owl:onProperty      <http://lbd.arch.rwth-aachen.de/bcf/v2.1/hasProjectId>
                         ] ;
        rdfs:subClassOf  [ a                   owl:Restriction ;
                           owl:minCardinality  "0"^^xsd:int ;
                           owl:onProperty      <http://lbd.arch.rwth-aachen.de/bcf/v2.1/hasProjectId>
                         ] .

<http://lbd.arch.rwth-aachen.de/bcf/v2.1/hasFileReference>
        a             owl:ObjectProperty ;
        rdfs:comment  "URI to IfcFile."@en ;
        rdfs:domain   <http://lbd.arch.rwth-aachen.de/bcf/v2.1/Header> .

<http://lbd.arch.rwth-aachen.de/bcf/v2.1/Lines>
        a             owl:Class ;
        rdfs:comment  "Lines can be used to add markup in 3D. Each line is defined by three dimensional Start Point and End Point. Lines that have the same start and end points are to be considered points and may be displayed accordingly."@en .

<http://lbd.arch.rwth-aachen.de/bcf/v2.1/hasHeader>
        a            owl:ObjectProperty ;
        rdfs:domain  <http://lbd.arch.rwth-aachen.de/bcf/v2.1/Markup> ;
        rdfs:range   <http://lbd.arch.rwth-aachen.de/bcf/v2.1/Header> .

<http://lbd.arch.rwth-aachen.de/bcf/v2.1/Camera>
        a                owl:Class ;
        rdfs:subClassOf  [ a                   owl:Restriction ;
                           owl:minCardinality  "1"^^xsd:int ;
                           owl:onProperty      <http://lbd.arch.rwth-aachen.de/bcf/v2.1/hasCameraUpVector>
                         ] ;
        rdfs:subClassOf  [ a                   owl:Restriction ;
                           owl:minCardinality  "1"^^xsd:int ;
                           owl:onProperty      <http://lbd.arch.rwth-aachen.de/bcf/v2.1/hasCameraDirection>
                         ] ;
        rdfs:subClassOf  [ a                   owl:Restriction ;
                           owl:minCardinality  "1"^^xsd:int ;
                           owl:onProperty      <http://lbd.arch.rwth-aachen.de/bcf/v2.1/hasCameraViewPoint>
                         ] .

<http://lbd.arch.rwth-aachen.de/bcf/v2.1/hasDescription>
        a             owl:DatatypeProperty , owl:ObjectProperty ;
        rdfs:comment  "Description of the document"@en , "Description of the topic."@en ;
        rdfs:domain   <http://lbd.arch.rwth-aachen.de/bcf/v2.1/DocumentReference> , <http://lbd.arch.rwth-aachen.de/bcf/v2.1/Topic> ;
        rdfs:range    xsd:string .

<http://lbd.arch.rwth-aachen.de/bcf/v2.1/hasFieldOfView>
        a             owl:ObjectProperty ;
        rdfs:comment  "Cameraâ€™s field of view angle in degrees."@en ;
        rdfs:domain   <http://lbd.arch.rwth-aachen.de/bcf/v2.1/PerspectiveCamera> .

<http://lbd.arch.rwth-aachen.de/bcf/v2.1/Markup>
        a       owl:Class .

<http://lbd.arch.rwth-aachen.de/bcf/v2.1/VisualizationInfo>
        a                owl:Class ;
        rdfs:subClassOf  [ a                   owl:Restriction ;
                           owl:minCardinality  "0"^^xsd:int ;
                           owl:onProperty      <http://lbd.arch.rwth-aachen.de/bcf/v2.1/hasPerspectiveCamera>
                         ] ;
        rdfs:subClassOf  [ a                   owl:Restriction ;
                           owl:minCardinality  "0"^^xsd:int ;
                           owl:onProperty      <http://lbd.arch.rwth-aachen.de/bcf/v2.1/hasOrthogonalCamera>
                         ] .

<http://lbd.arch.rwth-aachen.de/bcf/v2.1/hasOrthogonalCamera>
        a            owl:ObjectProperty ;
        rdfs:domain  <http://lbd.arch.rwth-aachen.de/bcf/v2.1/VisualizationInfo> ;
        rdfs:range   <http://lbd.arch.rwth-aachen.de/bcf/v2.1/OrthogonalCamera> .

<http://lbd.arch.rwth-aachen.de/bcf/v2.1/hasAuthor>
        a             owl:ObjectProperty ;
        rdfs:comment  "Comment author"@en ;
        rdfs:domain   <http://lbd.arch.rwth-aachen.de/bcf/v2.1/Comment> .

<http://lbd.arch.rwth-aachen.de/bcf/v2.1/hasOriginatingSystem>
        a             owl:ObjectProperty ;
        rdfs:comment  "Name of the system in which the component is originated"@en ;
        rdfs:domain   <http://lbd.arch.rwth-aachen.de/bcf/v2.1/Component> .

<http://lbd.arch.rwth-aachen.de/bcf/v2.1/Component>
        a       owl:Class .

<http://lbd.arch.rwth-aachen.de/bcf/v2.1/hasVisualizationInfo>
        a            owl:ObjectProperty ;
        rdfs:domain  <http://lbd.arch.rwth-aachen.de/bcf/v2.1/BCF> ;
        rdfs:range   <http://lbd.arch.rwth-aachen.de/bcf/v2.1/VisualizationInfo> .

<http://lbd.arch.rwth-aachen.de/bcf/v2.1/hasReferencedDocument>
        a             owl:ObjectProperty ;
        rdfs:comment  "URI to document."@en ;
        rdfs:domain   <http://lbd.arch.rwth-aachen.de/bcf/v2.1/DocumentReference> .

<http://lbd.arch.rwth-aachen.de/bcf/v2.1/hasCameraUpVector>
        a             owl:ObjectProperty ;
        rdfs:comment  "Camera up vector"@en ;
        rdfs:domain   <http://lbd.arch.rwth-aachen.de/bcf/v2.1/Camera> .

<http://lbd.arch.rwth-aachen.de/bcf/v2.1/hasModifiedDate>
        a             owl:DatatypeProperty ;
        rdfs:comment  "The date when comment was modified"@en , "Date when the topic was last modified. Exists only when Topic has been modified after creation."@en ;
        rdfs:domain   <http://lbd.arch.rwth-aachen.de/bcf/v2.1/Comment> , <http://lbd.arch.rwth-aachen.de/bcf/v2.1/Topic> ;
        rdfs:range    xsd:dateTime .